src/program_proof/simplepb/apps/closed_proof.v
@@ -95,177 +95,6 @@ Proof.
 Qed.
  *)
 
-Definition kv_replica_main_crash_cond `{ekvG Σ} γsys fname γsrv1:=
-(λ hG : heapGS Σ, ∃ data',
-    (fname f↦ data') ∗ ▷ file_crash (own_Server_ghost_f γsys γsrv1) data')%I.
-
-Lemma wpr_kv_replica_main fname me configHost {Σ} {HKV: ekvG Σ}
-                               {HG} {HL}:
-  let hG : heapGS Σ := {| goose_globalGS := HG; goose_localGS := HL |} in
-  "Hinit" ∷ fname f↦[] -∗
-  wpr NotStuck ⊤ (kv_replica_main #(LitString fname) #me #configHost) (kv_replica_main #(LitString fname) #me #configHost) (λ _ : goose_lang.val, True)
-    (λ _ , True) (λ _ _, True).
-Proof.
-  Locate wpr.
-  Print wpr.
-   iIntros. iNamed.
-   iApply (idempotence_wpr with "[Hinit Hfile_crash] []").
-   {
-     instantiate (1:=kv_replica_main_crash_cond γsys fname γsrv).
-     simpl.
-     wpc_apply (wpc_kv_replica_main γsys γsrv with "[] [$] [$] [$] [$]").
-     { iIntros "$". }
-     iExists _. iFrame.
-   }
-   { (* recovery *)
-     rewrite /hG.
-     clear hG.
-     iModIntro.
-     iIntros (????) "Hcrash".
-     iNext.
-     iDestruct "Hcrash" as (?) "[Hfile Hcrash]".
-     simpl.
-     set (hG' := HeapGS _ _ hL').
-     iDestruct "Hinvs" as "-#Hinvs".
-     iDestruct "Hsrvhost1" as "-#Hsrvhost1".
-     iDestruct "Hconfhost" as "-#Hconfhost".
-     iDestruct "Hproph" as "-#Hproph".
-     iCrash.
-     iIntros "_".
-     destruct hL as [HG'' ?].
-     iSplit; first done.
-     iDestruct "Hsrvhost1" as "(%&Hsrvhost1)".
-     iDestruct "Hconfhost" as "(%&Hconfhost)".
-     iDestruct "Hproph" as "(%&Hproph)".
-     subst.
-     clear hG'.
-     clear hL'.
-     (* overcome impedence mismatch between heapGS (bundled) and gooseGLobalGS+gooseLocalGS (split) proofs *)
-     set (hG2' := HeapGS _ _ goose_localGS).
-     simpl.
-     wpc_apply (wpc_kv_replica_main (heapGS0:=hG2') γsys γsrv with "[] [$] [$] [$] [$]").
-     { iIntros "H".
-       iDestruct "H" as (?) "[Hfile Hcrash]".
-       iExists _.
-       iFrame.
-     }
-     iExists _. iFrame.
-   }
-Qed.
-
-Lemma wp_lconfig_main γconf {Σ} {HKV: ekvG Σ} {HG} {HL} fname γ γsrv wf someN
-      (pPwf:configParams.Pwf.t Σ) (pNtop:configParams.Ntop.t)
-  :
-  let initconfig := configParams.initconfig.mk [lr1Host ; lr2Host] in
-  let paxosParams := definitions.mpaxosParams.mk Σ [γsrv] initstate wf someN in
-  let hG := {| goose_globalGS := HG; goose_localGS := HL |} in
-  "#Hhost" ∷ is_config_host lconfigHost γconf -∗
-  "#HpaxosHost" ∷ definitions.is_mpaxos_host lconfigHostPaxos γ γsrv -∗
-  WP lconfig_main #(str fname) {{ _, True }}
-.
-Proof.
-  intros ???.
-  repeat iNamed 1.
-  wp_call.
-  wp_apply (wp_NewSlice).
-  iIntros (?) "Hsl".
-  wp_apply wp_ref_to.
-  { done. }
-  iIntros (servers_ptr) "Hservers".
-  wp_pures.
-
-  wp_apply (wp_LoadAt with "[$Hservers]").
-  iIntros "Hservers".
-  wp_apply (wp_SliceAppend with "Hsl").
-  iIntros (?) "Hsl".
-  wp_apply (wp_StoreAt with "[$Hservers]").
-  { done. }
-  iIntros "Hservers".
-
-  wp_apply (wp_LoadAt with "[$Hservers]").
-  iIntros "Hservers".
-  wp_apply (wp_SliceAppend with "Hsl").
-  iIntros (?) "Hsl".
-  wp_apply (wp_StoreAt with "[$Hservers]").
-  { done. }
-  iIntros "Hservers".
-
-  wp_apply (wp_LoadAt with "[$Hservers]").
-  iIntros "Hservers".
-  iDestruct (own_slice_to_small with "Hsl") as "Hsl".
-  rewrite replicate_0.
-  simpl.
-  wp_apply wp_mk_lconfig_hosts.
-  iIntros (?) "#Hhosts_sl".
-  iMod (readonly_alloc_1 with "Hsl") as "Hsl".
-  wp_apply (config_proof.wp_StartServer with "[Hsl]").
-  {
-    iFrame "Hsl". iFrame "Hhost".
-    instantiate (8:=[lconfigHost]).
-    iSplitR; first admit.
-    iSplitR; first admit.
-    iSplitR; first admit.
-    iSplitR.
-    { admit. } (* FIXME: parameters don't match *)
-    admit.
-  }
-  iIntros (?) "#Hissrv".
-  wp_apply (wp_Server__Serve with "[$]").
-  {
-    iFrame "Hissrv".
-  }
-  wp_pures.
-  done.
-Qed.
-
-Lemma wp_dconfig_main γconf {Σ} {HKV: ekvG Σ} {HG} {HL}:
-  let hG := {| goose_globalGS := HG; goose_localGS := HL |} in
-  "HconfInit" ∷ makeConfigServer_pre γconf [dr1Host; dr2Host] ∗
-  "#Hhost" ∷ is_config_host dconfigHost γconf -∗
-  WP dconfig_main #() {{ _, True }}
-.
-Proof.
-  intros ?.
-  iNamed 1.
-  wp_call.
-  wp_apply (wp_NewSlice).
-  iIntros (?) "Hsl".
-  wp_apply wp_ref_to.
-  { done. }
-  iIntros (servers_ptr) "Hservers".
-  wp_pures.
-
-  wp_apply (wp_LoadAt with "[$Hservers]").
-  iIntros "Hservers".
-  wp_apply (wp_SliceAppend with "Hsl").
-  iIntros (?) "Hsl".
-  wp_apply (wp_StoreAt with "[$Hservers]").
-  { done. }
-  iIntros "Hservers".
-
-  wp_apply (wp_LoadAt with "[$Hservers]").
-  iIntros "Hservers".
-  wp_apply (wp_SliceAppend with "Hsl").
-  iIntros (?) "Hsl".
-  wp_apply (wp_StoreAt with "[$Hservers]").
-  { done. }
-  iIntros "Hservers".
-
-  wp_apply (wp_LoadAt with "[$Hservers]").
-  iIntros "Hservers".
-  iDestruct (own_slice_to_small with "Hsl") as "Hsl".
-  rewrite replicate_0.
-  simpl.
-  wp_apply (config_proof.wp_MakeServer with "[$HconfInit $Hsl]").
-  iIntros (?) "#Hissrv".
-  wp_apply (wp_Server__Serve with "[$]").
-  {
-    iFrame "Hissrv".
-  }
-  wp_pures.
-  done.
-Qed.
-
 (* There's one of these in kvee_proof.v, so I got rid of this.
    This is probably a remnant of an older version of the proof in which the subG
    wasn't proven anywhere else.
@@ -309,13 +138,13 @@ Lemma kv_pb_boot :
   g.(global_world).(grove_net) !! lr2Host = Some (∅ : gset message) →
 
   grove_dist_adequate
-    [ {| init_thread := dconfig_main #() ; init_restart := of_val #(); init_local_state := σdconfig |} ;
-      {| init_thread := lconfig_main #() ; init_restart := of_val #(); init_local_state := σlconfig |}
-      ]
-    [(kv_replica_main #(LitString replica_fname) #(dr1Host:u64) #dconfigHost, σdsrv1);
-     (kv_replica_main #(LitString replica_fname) #(dr2Host:u64) #dconfigHost, σdsrv2);
-     (kv_replica_main #(LitString replica_fname) #(lr1Host:u64) #lconfigHost, σlsrv1);
-     (kv_replica_main #(LitString replica_fname) #(lr2Host:u64) #lconfigHost, σlsrv2);
+    []
+    [
+      (dconfig_main #(LitString replica_fname), σlsrv2); (* FIXME: this needs to be a separate state *)
+      (kv_replica_main #(LitString replica_fname) #(dr1Host:u64) #dconfigHost, σdsrv1);
+      (kv_replica_main #(LitString replica_fname) #(dr2Host:u64) #dconfigHost, σdsrv2);
+      (kv_replica_main #(LitString replica_fname) #(lr1Host:u64) #lconfigHost, σlsrv1);
+      (kv_replica_main #(LitString replica_fname) #(lr2Host:u64) #lconfigHost, σlsrv2);
 
      (bank_transferer_main #(), σbt);
      (bank_auditor_main #(), σba)
@@ -334,6 +163,20 @@ Proof.
   iSplitR ""; last first.
   { iModIntro. iMod (fupd_mask_subseteq ∅); eauto. }
 
+  (* Allocate a vkv system *)
+  iMod (alloc_vkv [dr1Host ; dr2Host ] [(dconfigHost, dconfigHostPaxos)]
+                  {[ "init"; "a1"; "a2" ]} with "[Hchan]") as "[Hdkv Hdconf]".
+  { admit. }
+  iDestruct "Hdkv" as (γd ?)  "(Hkvs & #Hdhost & Hdsrvs)".
+  iSimpl in "Hdhost".
+
+  iMod (alloc_vkv [lr1Host ; lr2Host ] [(lconfigHost, lconfigHostPaxos)]
+                  {[ "init"; "a1"; "a2" ]} with "[]") as "[Hlkv Hlconf]".
+  { admit. }
+  iDestruct "Hlkv" as (γl ?)  "(Hlkvs & #Hlhost & Hlsrvs)".
+  iSimpl in "Hlhost".
+
+  (*
   (* SET UP RSM SYTEM *)
   (* First, pre-set up the two pairs of KV replica servers *)
   iMod (prealloc_simplepb_server) as (γsrvd1) "[#Hdsrv1wit Hdsrv1]".
@@ -417,21 +260,21 @@ Proof.
 
   iAssert (is_pb_config_host lconfigHost γlpb) with "[]" as "#HlConfHost".
   { iExists _. iFrame "#". }
-  (* END SET UP RSM SYTEM *)
+  (* END SET UP RSM SYTEM *) *)
 
   (* set up bank *)
   iAssert (|={⊤}=> is_bank "init" _ _ {[ "a1" ; "a2" ]})%I with "[Hlkvs Hkvs]" as ">#Hbank".
   {
     iDestruct (big_sepS_delete _ _ "init" with "Hlkvs") as "(Hinit&Hlkvs)".
     { set_solver. }
-    instantiate (2:=Build_lock_names (kv_ptsto γkv0)).
+    instantiate (2:=Build_lock_names (kv_ptsto γl)).
     rewrite /is_bank.
-    iMod (lock_alloc lockN {| kvptsto_lock := kv_ptsto γkv0 |} _ "init" with "[Hinit] [-]") as "$"; last done.
+    iMod (lock_alloc lockN {| kvptsto_lock := kv_ptsto γl |} _ "init" with "[Hinit] [-]") as "$"; last done.
     { iFrame. }
     iDestruct (big_sepS_delete _ _ "init" with "Hkvs") as "(Hinit&Hkvs)".
     { set_solver. }
     iLeft.
-    instantiate (1:=kv_ptsto γkv).
+    instantiate (1:=kv_ptsto γd).
     iFrame.
     iApply (big_sepS_sep).
     eassert (_ ∖ _ = {[ "a1"; "a2" ]}) as ->.
@@ -440,31 +283,19 @@ Proof.
   }
 
   iModIntro.
-  simpl. iSplitL "HconfInit".
+  iDestruct (big_sepL_cons with "Hdconf") as "[Hdconf _]".
+  simpl. iSplitL "Hdconf".
   {
     iIntros (HL) "Hfiles".
+    iDestruct (big_sepM_lookup_acc with "Hfiles") as "[Hfile _]".
+    { done. }
+    iDestruct "Hdconf" as (???) "(% & #Hhost & #Hpeers & #Hinvs & #Hwf & Hcrash)".
     iModIntro.
     iExists (λ _, True%I), (λ _, True%I), (λ _ _, True%I).
-    set (hG' := HeapGS _ _ _). (* overcome impedence mismatch between heapGS (bundled) and gooseGLobalGS+gooseLocalGS (split) proofs *)
-    iApply (idempotence_wpr with "[HconfInit] []").
-    {
-      instantiate (1:=λ _, True%I).
-      simpl.
-      iApply wp_wpc.
-      iApply (wp_dconfig_main _ with "[$]").
-    }
-    { (* crash; there should actually be no crashes of the config server *)
-      iModIntro.
-      iIntros.
-      iModIntro.
-      rewrite /post_crash.
-      iIntros. iModIntro.
-      iSplit; first done. iIntros. iSplit; first done.
-      set (hG2' := HeapGS _ _ _). (* overcome impedence mismatch between heapGS (bundled) and gooseGLobalGS+gooseLocalGS (split) proofs *)
-      wpc_pures.
-      { done. }
-      done.
-    }
+    set (hG' := HeapGS _ _ _).
+    iApply (wpr_dconfig_main with "[-]").
+    { done. }
+    { iFrame "∗#". }
   }
   iSplitL "HlconfInit".
   {
